---
layout: post
title: 4-27 å› å¼åˆ†è§£ä¸“é¢˜ç»ƒä¹ ç­”æ¡ˆ
permalink: /posts/2023/4/30/factorization-answer
---

é¢˜ç›®ğŸ“œï¼š[ğŸ”—](<{{ site.baseurl }}/posts/2023/4/28/factorization>)

ç­”æ¡ˆğŸ“ï¼š

1. åŸå¼ $ = 3 a b ^ { 2 } c ( a ^{ 2 } - 4 a c + 3 c ^ { 2 } ) \\ = 3 a b ^ { 2 } c ( a - 3 c ) ( a - c ) $
2. $ ( 4 x - 9 ) ( 4 x + 9 ) $
3. åŸå¼ $ = x ( y - 2 ) - 3 ( y - 2 ) \\ = ( x - 3 ) ( y - 2 ) $
4. $ ( x ^ { 2 } + y ^ { 2 } ) ( x - y ) $
5. $ ( 2 x - a ) ( x + b ) $
6. $ a ^ { 2 } ( a + 3 b ) ( a - 3 b ) $
7. åŸå¼ $ = x ^ { 3 } + 2 x ^ { 2 } + x ^ { 2 } - 4 \\ = x ^ { 2 } ( x + 2 ) + ( x + 2 ) ( x - 2 ) \\ = ( x + 2 ) ( x ^ { 2 } + x - 2 ) \\ = ( x + 2 ) ^ { 2 } ( x - 1 ) $
8. åŸå¼ $ = a b x ^ { 2 } + ( a ^ { 2 } - b ^ { 2 } ) x y - a b y ^ { 2 } \\ = ( a x - b y ) ( b x + a y ) $
9. åŸå¼ $ = ( x + y ) ( a - b - c ) - ( x - y ) ( a - b - c ) \\ = ( a - b - c ) ( x + y - x + y ) \\ = 2 y ( a - b - c ) $
10. åŸå¼ $ = a ^ { 2 } - b ^ { 2 } - ( a + b ) \\ = ( a - b ) ( a + b ) - ( a + b ) \\ = ( a + b ) ( a - b - 1 ) $
11. åŸå¼ $ = [ ( 3 a - b ) + 2 ( a + 3 b ) ] ^ { 2 } \\ = ( 5 a -5 b ) ^ { 2 } \\ = 25 ( a - b ) ^ { 2 } $
12. $ ( a + 3 ) ( a - 3 ) $
13. $ ( x + 1 ) ( x + 2 ) ( x + 1 - x - 2 ) \\ = - ( x + 1 ) ( x + 2 ) $
14. $ ( 3 x - 5 ) ^ { 2 } $
15. $ ( x - 10 ) ( x + 3 ) $
16. $ x ( x + 1 ) $
17. $ ( x - 4 ) ( x - a ) $
18. $ ( 5 x + 7 ) ( 5 x - 7 ) $
19. $ ( 6 x - 5 ) ^ { 2 } $
20. $ ( 2 x + 3 ) ^ { 2 } $
21. $ ( x - 3 ) ( x - 6 ) $
22. $ ( 2x - 3 ) ( x - 1 ) $
23. $ 2 ( x - 4 ) ( 6 x - 1 ) $
24. $ 3 x ( x - 2 ) $
25. $ ( 7 x - 5 ) ( 7 x + 5 ) $
26. $ ( 2 x - 1 ) ( 3 x - 5 ) $
27. $ ( x - 1 ) ( x + 3 ) $
28. $ ( 3 x + 8 ) ( 4 x - 3 ) $
29. $ ( x - 6 ) ( x + 5 ) $
30. åŸå¼ $ = ( x + 2 ) [ 3 ( x - 5 ) - x + 3 ] \\ = ( x + 2 ) ( 2 x -12 ) \\ = 2 ( x + 2 ) ( x - 6 ) $
31. $ ( 3 x + 7 ) ^ { 2 } $
32. $ x ^ { 2 } ( x - 7 ) ( x + 5 ) $
33. $ 3 x ^ { 2 } ( x ^ { 2 } + 1 ) ( x + 1 ) ( x - 1 ) $
34. $ ( x + 5 ) ( x - 5) $
35. $ ( x - 10 ) ^ { 2 } $
36. $ ( x + 1 ) ( x + 3 ) $
37. $ ( 2 x - 1 ) ( 2 x - 5 ) $
38. $ 3 a x ( x - 2 ) $
39. åŸå¼ $ = ( x + 2 ) ( x - 3 + x + 4 ) \\ = ( x + 2 ) ( x + 1 ) $
40. åŸå¼ $ = 2 a x ^ { 2 } + ( 2 a - 3 ) x -3 \\ = ( 2 a x - 3 ) ( x + 1 ) $
41. $ ( 3 x - 11 ) ^ { 2 } $
42. $ 2 ( 2 - x ) ( 2 + x ) $
43. $  $
44. 
